src/Context.v
@@ -2,7 +2,9 @@ Set Implicit Arguments.
 
 Require Import LibTactics.
 Require Import ListIds.
-Require Import Unify.
+Require Import Subst.
+Require Import SimpleTypes.
+Require Import MyLtacs.
 Require Import Disjoints.
 Require Import Schemes.
 Require Import Arith.Arith_base.
