src/Disjoints.v
@@ -1,7 +1,7 @@
 Set Implicit Arguments.
 
 Require Import ListIds.
-Require Import Unify.
+Require Import SimpleTypes.
 Require Import Arith.Arith_base List Omega.
 Require Import Wellfounded.Lexicographic_Product.
 Require Import Relation_Operators.
