src/MyLtacs.v
@@ -1,0 +1,21 @@
+Require Import LibTactics.
+Require Import Arith.Arith_base List Omega.
+Require Import SimpleTypes.
+
+Ltac s :=
+  match goal with
+    | [ H : _ /\ _ |- _] => destruct H
+    | [ H : _ \/ _ |- _] => destruct H
+    | [ |- context[eq_id_dec ?a ?b] ] => destruct (eq_id_dec a b) ; subst ; try congruence
+    | [ |- context[eq_nat_dec ?a ?b] ] => destruct (eq_nat_dec a b) ; subst ; try congruence
+    | [ x : (id * ty)%type |- _ ] => let t := fresh "t" in destruct x as [x t]
+    | [ H : (_,_) = (_,_) |- _] => inverts* H
+    | [ H : Some _ = Some _ |- _] => inverts* H
+    | [ H : Some _ = None |- _] => congruence
+    | [ H : None = Some _ |- _] => congruence
+    | [ |- _ /\ _] => split ~
+    | [ H : ex _ |- _] => destruct H
+  end.
+
+Ltac mysimp := (repeat (simpl; s)) ; simpl; auto with arith.
+
