src/NewTypeVariable.v
@@ -1,8 +1,11 @@
 Set Implicit Arguments.
 
-Require Import Unify.
+Require Import SimpleTypes.
+Require Import Omega.
 Require Import Schemes.
 Require Import List.
+Require Import MyLtacs.
+Require Import Subst.
 Require Import ListIds.
 Require Import Context.
 Require Import Relation_Operators.
@@ -17,6 +20,8 @@ Inductive new_tv_ty : ty -> id -> Prop :=
                                              new_tv_ty tau' i ->
                                              new_tv_ty (arrow tau tau') i.
 
+Hint Constructors new_tv_ty.
+
 Inductive new_tv_schm : schm -> id -> Prop :=
 | new_tv_sc_con : forall i i' : id, new_tv_schm (sc_con i') i
 | new_tv_sc_var : forall i i' : id, i < i' -> new_tv_schm (sc_var i) i'
@@ -25,6 +30,8 @@ Inductive new_tv_schm : schm -> id -> Prop :=
                                                new_tv_schm tau' i ->
                                                new_tv_schm (sc_arrow tau tau') i.
 
+Hint Constructors new_tv_schm.
+
 Inductive new_tv_ctx : ctx -> id -> Prop :=
 | new_tv_ctx_nil : forall i : id, new_tv_ctx nil i
 | new_tv_ctx_cons : forall (G : ctx) (i x : id) (sigma : schm),
@@ -32,15 +39,137 @@ Inductive new_tv_ctx : ctx -> id -> Prop :=
                             new_tv_schm sigma i ->
                             new_tv_ctx ((x, sigma) :: G) i.
 
+Hint Constructors new_tv_ctx.
+
 Inductive new_tv_subst : substitution -> id -> Prop :=
 | new_tv_subst_intro : forall (i : id) (s : substitution),
                   (forall x : id, in_list_id x (FV_subst s) = true -> x < i) ->
                   new_tv_subst s i.
 
+Hint Constructors new_tv_subst.
 
 Lemma new_tv_compose_subst : forall (s1 s2 : substitution) (i : id),
                              new_tv_subst s1 i ->
                              new_tv_subst s2 i ->
-                             new_tv_subst (s1 ++ s2) i.
+                             new_tv_subst (compose_subst s1 s2) i.
 Admitted.
+
+Hint Resolve new_tv_compose_subst.
+
+Lemma new_tv_subst_nil : forall st, new_tv_subst nil st.
+Proof.
+  intros. econstructor; intros ; simpl in *; inversion H.
+Qed.
+
+Hint Resolve new_tv_subst_nil.
+
+Lemma new_tv_schm_to_new_tv_ty : forall sigma x x0 i, new_tv_schm sigma x ->
+                          apply_inst_subst (compute_inst_subst x i) sigma = Some_schm x0 ->
+                          new_tv_ty x0 (x + i).
+Proof.
+  induction sigma; intros; simpl in *; mysimp.
+  - inversion H. inversion H0. econstructor. omega.
+  - inversion H0.  econstructor.
+  - pose proof (Nat.lt_ge_cases i0 i).
+    destruct H1.
+    + erewrite nth_error_compute_inst_None in H0; auto. 
+      inversion H0.
+    + apply Nat.lt_eq_cases in H1.
+      destruct H1.
+      * erewrite nth_error_compute_inst_Some in H0; auto.
+        inversion H0. inversion H.
+        subst.
+        econstructor.
+        omega.
+      * subst.
+        rewrite nth_error_compute_inst_None' in H0.
+        inversion H0.
+  - inversion H.
+    subst.
+    cases (apply_inst_subst (compute_inst_subst x i) sigma1).
+    cases (apply_inst_subst (compute_inst_subst x i) sigma2).
+    inversion H0.
+    econstructor; eauto. 
+    inversion H0.
+    inversion H0.
+Qed.
+
+Hint Resolve new_tv_schm_to_new_tv_ty.
+
+Lemma new_tv_subst_trans : forall (s : substitution) (i1 i2 : id),
+  new_tv_subst s i1 -> i1 <= i2 -> new_tv_subst s i2.
+Admitted.
+
+Hint Resolve new_tv_subst_trans.
+
+Lemma new_tv_s_id : forall (st st' : id) (s : substitution),
+    new_tv_subst s st -> st' < st -> new_tv_ty (apply_subst s (var st')) st.
+Admitted.
+
+Hint Resolve new_tv_s_id.
+
+Lemma new_tv_s_ty : forall (st : id) (s : substitution) (tau : ty),
+    new_tv_ty tau st -> new_tv_subst s st -> new_tv_ty (apply_subst s tau) st.
+Admitted.
+
+Hint Resolve new_tv_s_ty.
+
+Lemma new_tv_var_id : forall st1 st2 : id, st1 < st2 -> new_tv_ty (var st1) st2.
+Admitted.
+
+Hint Resolve new_tv_var_id.
+
+Lemma new_tv_ty_ids : forall (st : id) (tau : ty), new_tv_ty tau st ->
+                                               forall x : id, in_list_id x (ids_ty tau) = true -> x < st.
+Proof.
+  induction tau; intros; simpl in *; mysimp; intuition.
+  destruct (eq_id_dec i x); intuition. inversion H. omega.
+  apply in_list_id_or_append_inversion in H0.
+  destruct H0; inversion H; auto.
+Qed.
+
+Hint Resolve new_tv_ty_ids.
+
+Lemma new_tv_ty_trans_le : forall (tau : ty) (st1 st2 : id), new_tv_ty tau st1 -> st1 <= st2 -> new_tv_ty tau st2.
+Proof.
+  intros.
+  Admitted.
+
+Hint Resolve new_tv_ty_trans_le.
+
+Lemma new_tv_compose_subst_ctx : forall (s s1 s2 : substitution) (st : id) (G : ctx),
+       (forall x : id, x < st -> apply_subst s (var x) = apply_subst s2 (apply_subst s1 (var x))) ->
+       new_tv_ctx G st -> apply_subst_ctx s G = apply_subst_ctx s2 (apply_subst_ctx s1 G).
+Admitted.
+
+Lemma new_tv_schm_plus : forall sigma st st', new_tv_schm sigma st -> new_tv_schm sigma (st + st').
+Proof.
+  induction sigma; intros; try econstructor; eauto.
+  inversion H. subst. auto.
+  inversion H. subst. eauto.
+  Unshelve. apply x.
+Qed.
+
+Hint Resolve new_tv_schm_plus.
+
+Lemma new_tv_ctx_plus : forall G st st', new_tv_ctx G st -> new_tv_ctx G (st + st').
+Proof.
+  induction G; intros; simpl in *; auto.
+  destruct a.
+  econstructor; auto.
+  inversion H. subst;
+  eauto.
+  inversion H. subst;
+  eauto.
+Qed.
+
+Hint Resolve new_tv_ctx_plus.
+
+Lemma new_tv_ty_to_schm : forall tau st, new_tv_schm (ty_to_schm tau) st -> new_tv_ty tau st.
+Proof.
+  intros.
+  induction tau; simpl in *; try inversion H; try econstructor; eauto.
+Qed.
+
+Hint Resolve new_tv_ty_to_schm.
 
