src/SimpleTypes.v
@@ -1,0 +1,38 @@
+Set Implicit Arguments.
+
+Require Import Arith.Arith_base List Omega.
+
+(** * Type Definitions *)
+
+(** ** Identifier definition *)
+
+(** Identifiers are just natural numbers. This eases the task of equality test *)
+
+Definition id := nat.
+
+(** Decidable equality of identifiers *)
+
+Definition eq_id_dec : forall (v v' : id), {v = v'} + {v <> v'} := eq_nat_dec.
+
+(** Type definition is direct *)
+
+Inductive ty : Set :=
+  | var : id -> ty
+  | con : id -> ty
+  | arrow : ty -> ty -> ty.
+
+(** List of ids in a type *)
+Fixpoint ids_ty(tau : ty) : list id :=
+  match tau with
+  | var i => i::nil
+  | arrow l r => (ids_ty l) ++ (ids_ty r) 
+  | _ => nil
+  end.
+
+(** Decidable equality test for types *)
+
+Definition eq_ty_dec : forall (t t' : ty), {t = t'} + {t <> t'}.
+  pose eq_id_dec.
+  decide equality.
+Defined.
+
