src/Subst.v
@@ -1,0 +1,165 @@
+Set Implicit Arguments.
+
+Require Import Arith.Arith_base List Omega.
+Require Import Wellfounded.Lexicographic_Product.
+Require Import Relation_Operators.
+Require Import Coq.Setoids.Setoid.
+Require Import Program.
+Require Import SimpleTypes.
+Require Import LibTactics.
+Require Import MyLtacs.
+
+(** * Substitutions *)
+
+(** A operation for substitute all the ocurrences of variable x in t2 by t1. *)
+Definition substitution := list (id * ty).
+
+Fixpoint find_subst (s : substitution) (i : id) : option ty :=
+  match s with
+    | nil => None
+    | (v,t') :: s' => if (eq_id_dec v i) then Some t' else find_subst s' i
+  end.
+
+Fixpoint apply_subst (s : substitution) (t : ty) : ty :=
+  match t with
+  | arrow l r => arrow (apply_subst s l) (apply_subst s r)
+  | var i => match find_subst s i with
+            | None => var i
+            | Some t' => t'
+            end
+  | con i => con i
+  end.
+
+(** ** Substitution Definitions and Its Well Formedness Predicate *)
+
+(** Substitution and its dom *)
+
+Definition dom (s : substitution) : list id := List.map (@fst id ty) s.
+Definition img (s : substitution) : list ty := List.map (@snd id ty) s.
+Definition img_ids (s : substitution) : list id := List.concat (List.map ids_ty (img s)).
+
+(** ** Some Obvious Facts About Substitutions **)
+
+Lemma apply_subst_id : forall t, apply_subst nil t = t.
+Proof.
+  induction t ; mysimp.
+  congruence.
+Qed.
+
+Hint Resolve apply_subst_id.
+Hint Rewrite apply_subst_id : subst.
+
+Lemma apply_subst_con : forall s n, apply_subst s (con n) = con n.
+Proof.
+  induction s ; mysimp.
+Qed.
+
+Hint Resolve apply_subst_con.
+Hint Rewrite apply_subst_con : subst.
+
+Lemma apply_subst_arrow : forall s l r, apply_subst s (arrow l r) = arrow (apply_subst s l) (apply_subst s r).
+Proof.
+  induction s ; mysimp.
+Qed.
+
+Hint Resolve apply_subst_arrow.
+Hint Rewrite apply_subst_arrow : subst.
+
+(** ** Substitution composition **)
+Fixpoint in_subst_b (i : id) (s : substitution) : bool :=
+  match s with
+  | nil => false
+  | (j, _)::s' => if eq_id_dec i j then true else in_subst_b i s'
+  end.
+
+Fixpoint apply_subst_list (s1 s2 : substitution) : substitution :=
+  match s1 with
+  | nil => nil
+  | (i, t)::s1' => (i, apply_subst s2 t)::apply_subst_list s1' s2
+  end.
+
+Lemma apply_subst_nil : forall t, apply_subst nil t = t.
+Proof.
+  intros; induction t; mysimp.
+  congruence.
+Qed.
+
+Hint Resolve apply_subst_nil.
+Hint Rewrite apply_subst_nil : subst.
+
+Lemma apply_subst_list_nil : forall s, apply_subst_list s nil = s.
+Proof.
+  induction s; mysimp.
+  rewrite apply_subst_nil.
+  congruence.
+Qed.
+
+Hint Resolve apply_subst_list_nil.
+Hint Rewrite apply_subst_list_nil : subst.
+
+Definition compose_subst (s1 s2 : substitution) :=
+      apply_subst_list s1 s2 ++ s2.
+
+Lemma compose_subst_nil_l : forall s2, compose_subst nil s2 = s2.
+Proof.
+  intros; induction s2; mysimp.
+Qed.
+
+Hint Resolve compose_subst_nil_l.
+Hint Rewrite compose_subst_nil_l : subst.
+
+(** ** Some Obvious Facts About Composition **)
+
+Lemma apply_compose_subst_nil_l : forall s t, apply_subst (compose_subst nil s) t = apply_subst s t.
+Proof.
+  intros; mysimp. 
+Qed.
+
+Hint Resolve apply_compose_subst_nil_l.
+Hint Rewrite apply_compose_subst_nil_l : subst.
+
+Lemma apply_compose_subst_nil_r : forall s t, apply_subst (compose_subst s nil) t = apply_subst s t.
+Proof.
+  intros; mysimp; induction s; autorewrite with subst using congruence.
+  induction t; mysimp.
+  repeat rewrite apply_subst_arrow in IHs.
+  inversion IHs.
+  fequals;
+  auto.
+Qed.
+
+Hint Resolve apply_compose_subst_nil_r.
+Hint Rewrite apply_compose_subst_nil_r : subst.
+
+Lemma apply_subst_fold : forall s, (forall i, match find_subst s i with | Some t' => t' | None => var i end = apply_subst s (var i)).
+Proof.
+  intros. reflexivity.
+Qed.
+
+Lemma apply_subst_fold2 :  forall s s', (forall i, match find_subst s i with | Some t' => t' | None => var i end =
+                                         match find_subst s' i with | Some t' => t' | None => var i end) <->
+                                   (forall i, apply_subst s (var i) = apply_subst s' (var i)).
+Proof.
+  intros; split; intro; 
+    simpl in *;
+    auto.
+Qed.
+
+Lemma apply_compose_equiv : forall s1 s2 t, apply_subst (compose_subst s1 s2) t = apply_subst s2 (apply_subst s1 t).
+Proof.
+  induction s1; intros; mysimp. repeat rewrite apply_compose_subst_nil_l.  autorewrite with subst using congruence.
+  induction t; mysimp; simpl in *; eauto.
+  repeat rewrite apply_subst_fold.
+  erewrite <- IHs1.
+  simpl.
+  unfold compose_subst. reflexivity.
+  fequals.
+Qed.
+
+Definition FV_subst (s: substitution) := ((dom s) ++ (img_ids s)).
+
+Fixpoint id_in_subst (i : id) (s : substitution) : option ty :=
+  match s with
+    | nil => None
+    | (i', tau)::s' => if eq_id_dec i i' then Some tau else id_in_subst i s'
+  end.
